WIP, More WIP, Yet more WIP

theories/Dot/fundamental.v
@@ -29,22 +29,27 @@ Section fundamental.
 
   (* Make proofs below more robust. *)
   Opaque setp sdstp sdtp sptp sstpi.
+  Lemma sSub_Eq' {Γ T U i j} :
+    V⟦ Γ ⟧* s⊨ V⟦ T ⟧, i <: V⟦ U ⟧, j ⊣⊢
+    V⟦ Γ ⟧* s⊨ V⟦ iterate TLater i T ⟧, 0 <: V⟦ iterate TLater j U ⟧, 0.
+  Proof. by rewrite sSub_Eq !iterate_TLater_oLater. Qed.
 
   Definition fundamental_typed_def Γ g e T (HT: Γ v⊢ₜ[ g ] e : T) := ⊢ Γ ⊨[ Vs⟦ g ⟧ ] e : T.
   Definition fundamental_dms_typed_def Γ g ds T (HT: Γ v⊢ds[ g ] ds : T) := ⊢ Γ ⊨ds[ Vs⟦ g ⟧ ] ds : T.
   Definition fundamental_dm_typed_def Γ g l d T (HT : Γ v⊢[ g ]{ l := d } : T) := ⊢ Γ ⊨[ Vs⟦ g ⟧ ] { l := d } : T.
   Definition fundamental_path_typed_def Γ g p T i (HT : Γ v⊢ₚ[ g ] p : T, i) := ⊢ Γ ⊨p[ Vs⟦ g ⟧ ] p : T, i.
-  Definition fundamental_subtype_def Γ g T1 i1 T2 i2 (HT: Γ v⊢ₜ[ g ] T1, i1 <: T2, i2) :=
-    ⊢ Γ ⊨[ Vs⟦ g ⟧ ] T1, i1 <: T2, i2.
+  Definition fundamental_subtype_def Γ g T1 T2 (HT: Γ v⊢ₜ[ g ] T1 <: T2) :=
+    ⊢ Γ ⊨[ Vs⟦ g ⟧ ] T1, 0 <: T2, 0.
+  Arguments fundamental_subtype_def /.
 
   Theorem fundamental_mut Γ g :
     (∀ e T HT, @fundamental_typed_def Γ g e T HT) ∧
     (∀ ds T HT, @fundamental_dms_typed_def Γ g ds T HT) ∧
     (∀ l d T HT, @fundamental_dm_typed_def Γ g l d T HT) ∧
     (∀ p T i HT, @fundamental_path_typed_def Γ g p T i HT) ∧
-    (∀ T1 i1 T2 i2 HT, @fundamental_subtype_def Γ g T1 i1 T2 i2 HT).
+    (∀ T1 T2 HT, @fundamental_subtype_def Γ g T1 T2 HT).
   Proof.
-    apply storeless_typing_mut_ind; clear Γ g; intros; iIntros "#Hm".
+    apply storeless_typing_mut_ind; clear Γ g; intros; iIntros "#Hm"; rewrite -1?Sub_Eq.
       + by iApply T_All_Ex; [iApply H|iApply H0].
       + by iApply T_All_Ex_p; [|iApply H|iApply H0].
       + by iApply T_All_E; [iApply H|iApply H0].
@@ -55,7 +60,7 @@ Section fundamental.
       + iApply T_Obj_I. by iApply H.
       + iApply T_Mu_I. by iApply H.
       + by iApply T_Var.
-      + by iApply T_Sub; [iApply H0|iApply H].
+      + by iApply T_Sub; [iApply H0| rewrite Sub_Eq; iApply H].
       + iApply T_Path. by iApply H.
       + by iApply sT_Nat_I.
       + by iApply sT_Bool_I.
@@ -75,7 +80,7 @@ Section fundamental.
 
       + iApply P_Val. by iApply H.
       + iApply P_Fld_E. by iApply H.
-      + by iApply sP_Sub; [iApply H0|iApply H].
+      + by iApply sP_Sub; [iApply H0|rewrite sSub_Eq'; iApply H].
       + by iApply P_Mu_I; [|iApply H].
       + by iApply P_Mu_E; [|iApply H].
       + iApply P_Fld_I. by iApply H.
@@ -85,7 +90,7 @@ Section fundamental.
       + by iApply P_Sngl_E; [iApply H|iApply H0].
 
       + by iApply sSub_Refl.
-      + by iApply sSub_Trans; [iApply H|iApply H0].
+      + rewrite Sub_Eq. by iApply sSub_Trans; [iApply H|iApply H0].
       + by iApply sLater_Sub.
       + by iApply sSub_Later.
       + by iApply sSub_Add_Later.
@@ -93,21 +98,21 @@ Section fundamental.
       + by iApply sBot_Sub.
       + by iApply sAnd1_Sub.
       + by iApply sAnd2_Sub.
-      + by iApply sSub_And; [iApply H|iApply H0].
+      + by iApply sSub_And; rewrite sSub_Eq'; [iApply H|iApply H0].
       + by iApply sSub_Or1.
       + by iApply sSub_Or2.
-      + by iApply sOr_Sub; [iApply H|iApply H0].
+      + by iApply sOr_Sub; rewrite sSub_Eq'; [iApply H|iApply H0].
       + iApply sSel_Sub; by iApply H.
       + iApply sSub_Sel; by iApply H.
       + by iApply Sngl_pq_Sub; [|iApply H].
-      + by iApply Sngl_Sub_Sym; [iApply H|iApply H0].
+      + by iApply Sngl_Sub_Sym; rewrite 1?Sub_Eq; [iApply H| iApply H0].
       + iApply Sngl_Sub_Self. by iApply H.
-      + iApply Mu_Sub_Mu. by iApply H.
+      + iApply Mu_Sub_Mu. rewrite Sub_Eq. by iApply H.
       + iApply Mu_Sub.
       + iApply Sub_Mu.
-      + by iApply All_Sub_All; [iApply H|iApply H0].
-      + iApply Fld_Sub_Fld. by iApply H.
-      + by iApply Typ_Sub_Typ; [iApply H|iApply H0].
+      + by iApply All_Sub_All; rewrite 1?Sub_Eq; [iApply H|iApply H0].
+      + iApply Fld_Sub_Fld. rewrite Sub_Eq. by iApply H.
+      + by iApply Typ_Sub_Typ; rewrite 1?Sub_Eq; [iApply H|iApply H0].
       + iApply sAnd_All_Sub_Distr.
       + iApply sAnd_Fld_Sub_Distr.
       + iApply sAnd_Typ_Sub_Distr.
@@ -128,9 +133,13 @@ Section fundamental.
   Lemma fundamental_path_typed Γ g p T i :
     Γ v⊢ₚ[ g ] p : T, i → ⊢ Γ ⊨p[ Vs⟦ g ⟧ ] p : T, i.
   Proof. apply (fundamental_mut Γ g). Qed.
+  Lemma fundamental_subtype' Γ g T1 T2 :
+    Γ v⊢ₜ[ g ] T1 <: T2 → ⊢ Γ ⊨[ Vs⟦ g ⟧ ] T1, 0 <: T2, 0.
+  Proof. apply (fundamental_mut Γ g). Qed.
+
   Lemma fundamental_subtype Γ g T1 i1 T2 i2 :
     Γ v⊢ₜ[ g ] T1, i1 <: T2, i2 → ⊢ Γ ⊨[ Vs⟦ g ⟧ ] T1, i1 <: T2, i2.
-  Proof. apply (fundamental_mut Γ g). Qed.
+  Proof. rewrite Sub_Eq. apply fundamental_subtype'. Qed.
 End fundamental.
 
 (** Adequacy of our logical relation: semantically well-typed terms are safe. *)
